DynamoDbEncryption/runtimes/go/TestsFromDafny-go/awscryptographydbencryptionsdkdynamodbsmithygenerated/api_client.go
@@ -66,24 +66,3 @@ func (client *Client) GetEncryptedDataKeyDescription(ctx context.Context, params
 	return &native_response, nil
 
 }
-
-func (client *Client) GetNumberOfQueries(ctx context.Context, params awscryptographydbencryptionsdkdynamodbsmithygeneratedtypes.GetNumberOfQueriesInput) (*awscryptographydbencryptionsdkdynamodbsmithygeneratedtypes.GetNumberOfQueriesOutput, error) {
-	err := params.Validate()
-	if err != nil {
-		opaqueErr := awscryptographydbencryptionsdkdynamodbsmithygeneratedtypes.OpaqueError{
-			ErrObject: err,
-		}
-		return nil, opaqueErr
-	}
-
-	var dafny_request AwsCryptographyDbEncryptionSdkDynamoDbTypes.GetNumberOfQueriesInput = GetNumberOfQueriesInput_ToDafny(params)
-	var dafny_response = client.DafnyClient.GetNumberOfQueries(dafny_request)
-
-	if dafny_response.Is_Failure() {
-		err := dafny_response.Dtor_error().(AwsCryptographyDbEncryptionSdkDynamoDbTypes.Error)
-		return nil, Error_FromDafny(err)
-	}
-	var native_response = GetNumberOfQueriesOutput_FromDafny(dafny_response.Dtor_value().(AwsCryptographyDbEncryptionSdkDynamoDbTypes.GetNumberOfQueriesOutput))
-	return &native_response, nil
-
-}
