DynamoDbEncryption/runtimes/go/TestsFromDafny-go/awscryptographydbencryptionsdkdynamodbsmithygenerated/to_dafny.go
@@ -3,7 +3,6 @@
 package awscryptographydbencryptionsdkdynamodbsmithygenerated
 
 import (
-	"github.com/aws/aws-cryptographic-material-providers-library/releases/go/dynamodb/ComAmazonawsDynamodbTypes"
 	"github.com/aws/aws-cryptographic-material-providers-library/releases/go/dynamodb/comamazonawsdynamodbsmithygenerated"
 	"github.com/aws/aws-cryptographic-material-providers-library/releases/go/mpl/AwsCryptographyKeyStoreTypes"
 	"github.com/aws/aws-cryptographic-material-providers-library/releases/go/mpl/AwsCryptographyMaterialProvidersTypes"
@@ -20,7 +19,6 @@ import (
 	"github.com/aws/aws-database-encryption-sdk-dynamodb/releases/go/dynamodb-esdk/awscryptographydbencryptionsdkdynamodbsmithygeneratedtypes"
 	"github.com/aws/aws-database-encryption-sdk-dynamodb/releases/go/dynamodb-esdk/awscryptographydbencryptionsdkstructuredencryptionsmithygenerated"
 	"github.com/aws/aws-database-encryption-sdk-dynamodb/releases/go/dynamodb-esdk/awscryptographydbencryptionsdkstructuredencryptionsmithygeneratedtypes"
-	"github.com/aws/aws-sdk-go-v2/service/dynamodb"
 	dynamodbtypes "github.com/aws/aws-sdk-go-v2/service/dynamodb/types"
 	"github.com/aws/smithy-go"
 	"github.com/dafny-lang/DafnyRuntimeGo/v4/dafny"
@@ -58,24 +56,6 @@ func GetEncryptedDataKeyDescriptionOutput_ToDafny(nativeOutput awscryptographydb
 	return func() AwsCryptographyDbEncryptionSdkDynamoDbTypes.GetEncryptedDataKeyDescriptionOutput {
 
 		return AwsCryptographyDbEncryptionSdkDynamoDbTypes.Companion_GetEncryptedDataKeyDescriptionOutput_.Create_GetEncryptedDataKeyDescriptionOutput_(Aws_cryptography_dbEncryptionSdk_dynamoDb_GetEncryptedDataKeyDescriptionOutput_EncryptedDataKeyDescriptionOutput_ToDafny(nativeOutput.EncryptedDataKeyDescriptionOutput))
-	}()
-
-}
-
-func GetNumberOfQueriesInput_ToDafny(nativeInput awscryptographydbencryptionsdkdynamodbsmithygeneratedtypes.GetNumberOfQueriesInput) AwsCryptographyDbEncryptionSdkDynamoDbTypes.GetNumberOfQueriesInput {
-
-	return func() AwsCryptographyDbEncryptionSdkDynamoDbTypes.GetNumberOfQueriesInput {
-
-		return AwsCryptographyDbEncryptionSdkDynamoDbTypes.Companion_GetNumberOfQueriesInput_.Create_GetNumberOfQueriesInput_(Aws_cryptography_dbEncryptionSdk_dynamoDb_GetNumberOfQueriesInput_input_ToDafny(nativeInput.Input))
-	}()
-
-}
-
-func GetNumberOfQueriesOutput_ToDafny(nativeOutput awscryptographydbencryptionsdkdynamodbsmithygeneratedtypes.GetNumberOfQueriesOutput) AwsCryptographyDbEncryptionSdkDynamoDbTypes.GetNumberOfQueriesOutput {
-
-	return func() AwsCryptographyDbEncryptionSdkDynamoDbTypes.GetNumberOfQueriesOutput {
-
-		return AwsCryptographyDbEncryptionSdkDynamoDbTypes.Companion_GetNumberOfQueriesOutput_.Create_GetNumberOfQueriesOutput_(Aws_cryptography_dbEncryptionSdk_dynamoDb_GetNumberOfQueriesOutput_numberOfQueries_ToDafny(nativeOutput.NumberOfQueries))
 	}()
 
 }
@@ -695,20 +675,6 @@ func Aws_cryptography_dbEncryptionSdk_dynamoDb_EncryptedDataKeyDescription_branc
 			}
 			return res
 		}())
-	}()
-}
-
-func Aws_cryptography_dbEncryptionSdk_dynamoDb_GetNumberOfQueriesInput_input_ToDafny(input dynamodb.QueryInput) ComAmazonawsDynamodbTypes.QueryInput {
-	return func() ComAmazonawsDynamodbTypes.QueryInput {
-
-		return ComAmazonawsDynamodbTypes.Companion_QueryInput_.Create_QueryInput_(comamazonawsdynamodbsmithygenerated.Com_amazonaws_dynamodb_QueryInput_TableName_ToDafny(input.TableName), comamazonawsdynamodbsmithygenerated.Com_amazonaws_dynamodb_QueryInput_IndexName_ToDafny(input.IndexName), comamazonawsdynamodbsmithygenerated.Com_amazonaws_dynamodb_QueryInput_Select_ToDafny(input.Select), comamazonawsdynamodbsmithygenerated.Com_amazonaws_dynamodb_QueryInput_AttributesToGet_ToDafny(input.AttributesToGet), comamazonawsdynamodbsmithygenerated.Com_amazonaws_dynamodb_QueryInput_Limit_ToDafny(input.Limit), comamazonawsdynamodbsmithygenerated.Com_amazonaws_dynamodb_QueryInput_ConsistentRead_ToDafny(input.ConsistentRead), comamazonawsdynamodbsmithygenerated.Com_amazonaws_dynamodb_QueryInput_KeyConditions_ToDafny(input.KeyConditions), comamazonawsdynamodbsmithygenerated.Com_amazonaws_dynamodb_QueryInput_QueryFilter_ToDafny(input.QueryFilter), comamazonawsdynamodbsmithygenerated.Com_amazonaws_dynamodb_QueryInput_ConditionalOperator_ToDafny(input.ConditionalOperator), comamazonawsdynamodbsmithygenerated.Com_amazonaws_dynamodb_QueryInput_ScanIndexForward_ToDafny(input.ScanIndexForward), comamazonawsdynamodbsmithygenerated.Com_amazonaws_dynamodb_QueryInput_ExclusiveStartKey_ToDafny(input.ExclusiveStartKey), comamazonawsdynamodbsmithygenerated.Com_amazonaws_dynamodb_QueryInput_ReturnConsumedCapacity_ToDafny(input.ReturnConsumedCapacity), comamazonawsdynamodbsmithygenerated.Com_amazonaws_dynamodb_QueryInput_ProjectionExpression_ToDafny(input.ProjectionExpression), comamazonawsdynamodbsmithygenerated.Com_amazonaws_dynamodb_QueryInput_FilterExpression_ToDafny(input.FilterExpression), comamazonawsdynamodbsmithygenerated.Com_amazonaws_dynamodb_QueryInput_KeyConditionExpression_ToDafny(input.KeyConditionExpression), comamazonawsdynamodbsmithygenerated.Com_amazonaws_dynamodb_QueryInput_ExpressionAttributeNames_ToDafny(input.ExpressionAttributeNames), comamazonawsdynamodbsmithygenerated.Com_amazonaws_dynamodb_QueryInput_ExpressionAttributeValues_ToDafny(input.ExpressionAttributeValues))
-	}()
-}
-
-func Aws_cryptography_dbEncryptionSdk_dynamoDb_GetNumberOfQueriesOutput_numberOfQueries_ToDafny(input int32) int32 {
-	return func() int32 {
-
-		return input
 	}()
 }
 
