DynamoDbEncryption/runtimes/java/src/main/smithy-generated/software/amazon/cryptography/dbencryptionsdk/dynamodb/ToDafny.java
@@ -39,8 +39,6 @@ import software.amazon.cryptography.dbencryptionsdk.dynamodb.internaldafny.types
 import software.amazon.cryptography.dbencryptionsdk.dynamodb.internaldafny.types.GetEncryptedDataKeyDescriptionInput;
 import software.amazon.cryptography.dbencryptionsdk.dynamodb.internaldafny.types.GetEncryptedDataKeyDescriptionOutput;
 import software.amazon.cryptography.dbencryptionsdk.dynamodb.internaldafny.types.GetEncryptedDataKeyDescriptionUnion;
-import software.amazon.cryptography.dbencryptionsdk.dynamodb.internaldafny.types.GetNumberOfQueriesInput;
-import software.amazon.cryptography.dbencryptionsdk.dynamodb.internaldafny.types.GetNumberOfQueriesOutput;
 import software.amazon.cryptography.dbencryptionsdk.dynamodb.internaldafny.types.GetPrefix;
 import software.amazon.cryptography.dbencryptionsdk.dynamodb.internaldafny.types.GetSegment;
 import software.amazon.cryptography.dbencryptionsdk.dynamodb.internaldafny.types.GetSegments;
@@ -76,7 +74,6 @@ import software.amazon.cryptography.materialproviders.internaldafny.types.IBranc
 import software.amazon.cryptography.materialproviders.internaldafny.types.ICryptographicMaterialsManager;
 import software.amazon.cryptography.materialproviders.internaldafny.types.IKeyring;
 import software.amazon.cryptography.services.dynamodb.internaldafny.types.AttributeValue;
-import software.amazon.cryptography.services.dynamodb.internaldafny.types.QueryInput;
 
 public class ToDafny {
 
@@ -619,25 +616,6 @@ public class ToDafny {
     return new GetEncryptedDataKeyDescriptionOutput(
       encryptedDataKeyDescriptionOutput
     );
-  }
-
-  public static GetNumberOfQueriesInput GetNumberOfQueriesInput(
-    software.amazon.cryptography.dbencryptionsdk.dynamodb.model.GetNumberOfQueriesInput nativeValue
-  ) {
-    QueryInput input;
-    input =
-      software.amazon.cryptography.services.dynamodb.internaldafny.ToDafny.QueryInput(
-        nativeValue.input()
-      );
-    return new GetNumberOfQueriesInput(input);
-  }
-
-  public static GetNumberOfQueriesOutput GetNumberOfQueriesOutput(
-    software.amazon.cryptography.dbencryptionsdk.dynamodb.model.GetNumberOfQueriesOutput nativeValue
-  ) {
-    Integer numberOfQueries;
-    numberOfQueries = (nativeValue.numberOfQueries());
-    return new GetNumberOfQueriesOutput(numberOfQueries);
   }
 
   public static GetPrefix GetPrefix(
