DynamoDbEncryption/runtimes/java/src/main/smithy-generated/software/amazon/cryptography/dbencryptionsdk/dynamodb/ToNative.java
@@ -40,8 +40,6 @@ import software.amazon.cryptography.dbencryptionsdk.dynamodb.model.GetBucketNumb
 import software.amazon.cryptography.dbencryptionsdk.dynamodb.model.GetEncryptedDataKeyDescriptionInput;
 import software.amazon.cryptography.dbencryptionsdk.dynamodb.model.GetEncryptedDataKeyDescriptionOutput;
 import software.amazon.cryptography.dbencryptionsdk.dynamodb.model.GetEncryptedDataKeyDescriptionUnion;
-import software.amazon.cryptography.dbencryptionsdk.dynamodb.model.GetNumberOfQueriesInput;
-import software.amazon.cryptography.dbencryptionsdk.dynamodb.model.GetNumberOfQueriesOutput;
 import software.amazon.cryptography.dbencryptionsdk.dynamodb.model.GetPrefix;
 import software.amazon.cryptography.dbencryptionsdk.dynamodb.model.GetSegment;
 import software.amazon.cryptography.dbencryptionsdk.dynamodb.model.GetSegments;
@@ -524,28 +522,6 @@ public class ToNative {
         dafnyValue.dtor_EncryptedDataKeyDescriptionOutput()
       )
     );
-    return nativeBuilder.build();
-  }
-
-  public static GetNumberOfQueriesInput GetNumberOfQueriesInput(
-    software.amazon.cryptography.dbencryptionsdk.dynamodb.internaldafny.types.GetNumberOfQueriesInput dafnyValue
-  ) {
-    GetNumberOfQueriesInput.Builder nativeBuilder =
-      GetNumberOfQueriesInput.builder();
-    nativeBuilder.input(
-      software.amazon.cryptography.services.dynamodb.internaldafny.ToNative.QueryInput(
-        dafnyValue.dtor_input()
-      )
-    );
-    return nativeBuilder.build();
-  }
-
-  public static GetNumberOfQueriesOutput GetNumberOfQueriesOutput(
-    software.amazon.cryptography.dbencryptionsdk.dynamodb.internaldafny.types.GetNumberOfQueriesOutput dafnyValue
-  ) {
-    GetNumberOfQueriesOutput.Builder nativeBuilder =
-      GetNumberOfQueriesOutput.builder();
-    nativeBuilder.numberOfQueries((dafnyValue.dtor_numberOfQueries()));
     return nativeBuilder.build();
   }
 
