DynamoDbEncryption/dafny/DynamoDbEncryption/Model/AwsCryptographyDbEncryptionSdkDynamoDbTypes.dfy
@@ -168,11 +168,9 @@ module {:extern "software.amazon.cryptography.dbencryptionsdk.dynamodb.internald
     ghost constructor() {
       CreateDynamoDbEncryptionBranchKeyIdSupplier := [];
       GetEncryptedDataKeyDescription := [];
-      GetNumberOfQueries := [];
     }
     ghost var CreateDynamoDbEncryptionBranchKeyIdSupplier: seq<DafnyCallEvent<CreateDynamoDbEncryptionBranchKeyIdSupplierInput, Result<CreateDynamoDbEncryptionBranchKeyIdSupplierOutput, Error>>>
     ghost var GetEncryptedDataKeyDescription: seq<DafnyCallEvent<GetEncryptedDataKeyDescriptionInput, Result<GetEncryptedDataKeyDescriptionOutput, Error>>>
-    ghost var GetNumberOfQueries: seq<DafnyCallEvent<GetNumberOfQueriesInput, Result<GetNumberOfQueriesOutput, Error>>>
   }
   trait {:termination false} IDynamoDbEncryptionClient
   {
@@ -241,21 +239,6 @@ module {:extern "software.amazon.cryptography.dbencryptionsdk.dynamodb.internald
         && ValidState()
       ensures GetEncryptedDataKeyDescriptionEnsuresPublicly(input, output)
       ensures History.GetEncryptedDataKeyDescription == old(History.GetEncryptedDataKeyDescription) + [DafnyCallEvent(input, output)]
-
-    predicate GetNumberOfQueriesEnsuresPublicly(input: GetNumberOfQueriesInput , output: Result<GetNumberOfQueriesOutput, Error>)
-    // The public method to be called by library consumers
-    method GetNumberOfQueries ( input: GetNumberOfQueriesInput )
-      returns (output: Result<GetNumberOfQueriesOutput, Error>)
-      requires
-        && ValidState()
-      modifies Modifies - {History} ,
-               History`GetNumberOfQueries
-      // Dafny will skip type parameters when generating a default decreases clause.
-      decreases Modifies - {History}
-      ensures
-        && ValidState()
-      ensures GetNumberOfQueriesEnsuresPublicly(input, output)
-      ensures History.GetNumberOfQueries == old(History.GetNumberOfQueries) + [DafnyCallEvent(input, output)]
 
   }
   datatype DynamoDbEncryptionConfig = | DynamoDbEncryptionConfig (
@@ -381,12 +364,6 @@ module {:extern "software.amazon.cryptography.dbencryptionsdk.dynamodb.internald
   datatype GetEncryptedDataKeyDescriptionUnion =
     | header(header: seq<uint8>)
     | item(item: ComAmazonawsDynamodbTypes.AttributeMap)
-  datatype GetNumberOfQueriesInput = | GetNumberOfQueriesInput (
-    nameonly input: ComAmazonawsDynamodbTypes.QueryInput
-  )
-  datatype GetNumberOfQueriesOutput = | GetNumberOfQueriesOutput (
-    nameonly numberOfQueries: BucketCount
-  )
   datatype GetPrefix = | GetPrefix (
     nameonly length: int32
   )
@@ -686,26 +663,6 @@ abstract module AbstractAwsCryptographyDbEncryptionSdkDynamoDbService
       History.GetEncryptedDataKeyDescription := History.GetEncryptedDataKeyDescription + [DafnyCallEvent(input, output)];
     }
 
-    predicate GetNumberOfQueriesEnsuresPublicly(input: GetNumberOfQueriesInput , output: Result<GetNumberOfQueriesOutput, Error>)
-    {Operations.GetNumberOfQueriesEnsuresPublicly(input, output)}
-    // The public method to be called by library consumers
-    method GetNumberOfQueries ( input: GetNumberOfQueriesInput )
-      returns (output: Result<GetNumberOfQueriesOutput, Error>)
-      requires
-        && ValidState()
-      modifies Modifies - {History} ,
-               History`GetNumberOfQueries
-      // Dafny will skip type parameters when generating a default decreases clause.
-      decreases Modifies - {History}
-      ensures
-        && ValidState()
-      ensures GetNumberOfQueriesEnsuresPublicly(input, output)
-      ensures History.GetNumberOfQueries == old(History.GetNumberOfQueries) + [DafnyCallEvent(input, output)]
-    {
-      output := Operations.GetNumberOfQueries(config, input);
-      History.GetNumberOfQueries := History.GetNumberOfQueries + [DafnyCallEvent(input, output)];
-    }
-
   }
 }
 abstract module AbstractAwsCryptographyDbEncryptionSdkDynamoDbOperations {
@@ -755,20 +712,4 @@ abstract module AbstractAwsCryptographyDbEncryptionSdkDynamoDbOperations {
     ensures
       && ValidInternalConfig?(config)
     ensures GetEncryptedDataKeyDescriptionEnsuresPublicly(input, output)
-
-
-  predicate GetNumberOfQueriesEnsuresPublicly(input: GetNumberOfQueriesInput , output: Result<GetNumberOfQueriesOutput, Error>)
-  // The private method to be refined by the library developer
-
-
-  method GetNumberOfQueries ( config: InternalConfig , input: GetNumberOfQueriesInput )
-    returns (output: Result<GetNumberOfQueriesOutput, Error>)
-    requires
-      && ValidInternalConfig?(config)
-    modifies ModifiesInternalConfig(config)
-    // Dafny will skip type parameters when generating a default decreases clause.
-    decreases ModifiesInternalConfig(config)
-    ensures
-      && ValidInternalConfig?(config)
-    ensures GetNumberOfQueriesEnsuresPublicly(input, output)
 }
